

Not having a good time with the `mathpartir` package here.

Exercise 4.1

Calls to `g` declare a reference `counter`, set its contents, then return its contents. The information between calls is lost because `counter` is different on each call. That is, the reference data structure represents a different location. The first program was made such that the environment of the closure had access to `counter`, and thus was able to reference that variable.

Exercise 4.2

$$\frac{(\text{value-of } \text{exp}_1 \ \rho \ \sigma_0) = (val_1, \sigma_1)}{(\text{value-of } (\text{zero?-exp } \text{exp}_1) \ \rho \ \sigma_0) = \begin{array}{ll} ((\text{bool-val } \#t), \sigma_1) & \text{if } [val_1] = 0 \\ ((\text{bool-val } \#f), \sigma_1) & \text{if } [val_1] \neq 0 \end{array}}$$

Exercise 4.3

$$\frac{\begin{array}{l} (\text{value-of } \text{exp}_1 \ \rho \ \sigma_0) = (val_1, \sigma_1) \\ (\text{value-of } \text{exp}_2 \ \rho \ \sigma_1) = (val_2, \sigma_2) \end{array}}{(\text{value-of } (\text{call-exp } \text{exp}_1 \ \text{exp}_2) \ \rho \ \sigma_0) = (\text{apply-procedure } (\text{expval} \rightarrow \text{proc } val_1) \ val_2 \ \sigma_2)}$$

$$\frac{val_1 = (\text{procedure } \text{var } \text{body } \rho)}{(\text{apply-procedure } val_1 \ val_2 \ \rho_0) = (\text{value-of } \text{body } [var = val_2] \rho \ \sigma_0)}$$

Exercise 4.4

$$\begin{array}{c}
(\text{value-of } exp_1 \ \rho \ \sigma_0) = (val_1, \sigma_1) \\
\vdots \\
(\text{value-of } exp_n \ \rho \ \sigma_{n-1}) = (val_n, \sigma_n) \\
\hline
(\text{value-of } (\text{begin } exp_1 \dots exp_n) \ \rho \ \sigma_0) = (val_n, \sigma_n)
\end{array}$$

Exercise 4.5

$$\begin{array}{c}
(\text{value-of } exp_1 \ \rho \ \sigma_0) = (val_1, \sigma_1) \\
\vdots \\
(\text{value-of } exp_n \ \rho \ \sigma_{n-1}) = (val_n, \sigma_n) \\
\hline
(\text{value-of } (\text{list-exp } exp_1 \dots exp_n) \ \rho \ \sigma_0) \\
= ((\text{pair-val } val_1 \ (\dots (\text{pair-val } val_n \ (\text{emptylist-val})) \dots)), \sigma_n)
\end{array}$$

Exercise 4.6

$$\begin{array}{c}
(\text{value-of } exp_1 \ \rho \ \sigma_0) = (l, \sigma_1) \\
(\text{value-of } exp_2 \ \rho \ \sigma_1) = (val, \sigma_2) \\
\hline
(\text{value-of } (\text{setref-exp } exp_1 \ exp_2) \ \rho \ \sigma_0) = (val, [l = val]\sigma_2)
\end{array}$$

Exercise 4.7

$$\begin{array}{c}
(\text{value-of } exp_1 \ \rho \ \sigma_0) = (l, \sigma_1) \\
(\text{value-of } exp_2 \ \rho \ \sigma_1) = (val, \sigma_2) \\
\hline
(\text{value-of } (\text{setref-exp } exp_1 \ exp_2) \ \rho \ \sigma_0) = (\sigma_0(l), [l = val]\sigma_2)
\end{array}$$